organize project

ContractEquations.v
@@ -1,69 +1,215 @@
 Require Import CSL.Contract.
+Require Import CSL.Order.
+Require Import Lists.List.
+Require Import Sorting.Permutation.
+Require Import Sorting.Mergesort.
+Require Import Sorting.Sorted.
+Require Import Bool.Bool.
+Require Import Bool.Sumbool.
+Require Import List Setoid Permutation Sorted Orders.
+Import ListNotations.
+
+Set Implicit Arguments.
+
+Module Import TraceSort := Sort TraceOrder.
 
 Reserved Notation "c0 =R= c1" (at level 63).
 
+Hint Constructors matches_comp : core.
+
 Inductive c_eq : Contract -> Contract -> Prop :=
-  | plus_assoc c0 c1 c2 : (c0 _+_ c1) _+_ c2 =R= c0 _+_ (c1 _+_ c2)
-  | plus_comm c0 c1: c0 _+_ c1 =R= c1 _+_ c0
-  | plus_neut c: c _+_ Failure =R= c
-  | seq_assoc c0 c1 c2 : (c0 _;_ c1) _;_ c2 =R= c0 _;_ (c1 _;_ c2)
-  | seq_neut c0 c1 c2 : (c0 _;_ ) _;_ c2 =R= c0 _;_ (c1 _;_ c2)
-  | distr_l c0 c1 c2 : c0 _;_ (c1 _+_ c2) =R= (c0 _+_ c1) _;_ (c0 _+_ c2)
-  | distr_r c0 c1 c2 : (c0 _+_ c1) _;_ c2 =R= (c0 _+_ c2) _;_ (c1 _+_ c2)
+  | c_plus_assoc c0 c1 c2 : (c0 _+_ c1) _+_ c2 =R= c0 _+_ (c1 _+_ c2)
+  | c_plus_comm c0 c1: c0 _+_ c1 =R= c1 _+_ c0
+  | c_plus_neut c: c _+_ Failure =R= c
+  | c_plus_idemp c : c _+_ c =R= c 
+  | c_seq_assoc c0 c1 c2 : (c0 _;_ c1) _;_ c2 =R= c0 _;_ (c1 _;_ c2)
+  | c_seq_neut_l c : (Success _;_ c) =R= c 
+  | c_seq_neut_r c : c _;_ Success =R= c 
+  | c_distr_l c0 c1 c2 : c0 _;_ (c1 _+_ c2) =R= (c0 _;_ c1) _+_ (c0 _;_ c2)
+  | c_distr_r c0 c1 c2 : (c0 _+_ c1) _;_ c2 =R= (c0 _;_ c2) _+_ (c1 _;_ c2)
+  | c_refl c : c =R= c
+  | c_sym c0 c1 (H: c0 =R= c1) : c1 =R= c0
+  | c_trans c0 c1 c2 (H1 : c0 =R= c1) (H2 : c1 =R= c2) : c0 =R= c2
   where "c1 =R= c2" := (c_eq c1 c2).
 
+Add Parametric Relation : Contract c_eq
+  reflexivity proved by c_refl
+  symmetry proved by c_sym
+  transitivity proved by c_trans
+  as Contract_setoid.
 
-  | plus_idem : Failure _+_ Failure =R= Failure
-
-
-
-
-Definition c_eq (c c':Contract) : Prop := forall s, s ==~ c <-> s ==~ c'.
-
-Notation "a =R= b" := (c_eq a b) (at level 70).
-
-
-Lemma plus_comm : forall (c1 c2 : Contract), (c1 _+_ c2) =R= (c2 _+_ c1).
+Lemma c_eq_soundness : forall (c0 c1 : Contract), c0 =R= c1 -> (forall s : Trace, s ==~ c0 <-> s ==~ c1).
 Proof.
-split ; intros ; inversion H ; auto.
+- intros. induction H.
+  * split ; intros ; inversion H; auto. all: inversion H2 ; auto. inversion H1 ; auto.
+  * split ; intros ; inversion H ; auto. 
+  * split ; intros ; inversion H ; auto. inversion H1.
+  * split ; intros ; inversion H ; auto.
+  * split ; intros ; inversion H ; auto. 
+    ** inversion H3. rewrite <- app_assoc. auto.
+    ** inversion H4. rewrite app_assoc. auto.
+  * split ; intros. 
+    **  inversion H. inversion H3. now assumption.
+    ** rewrite <- (app_nil_l s). auto. 
+  * split ; intros.
+    ** inversion H. inversion H4. rewrite app_nil_r. assumption.
+    ** rewrite <- (app_nil_r s). auto.
+  * split ; intros ; inversion H.
+    ** inversion H4 ; auto.
+    ** inversion H2 ; auto.
+    ** inversion H1 ; auto.
+  * split ; intros ; inversion H.
+    ** inversion H3 ; auto.
+    ** inversion H2 ; auto.
+    ** inversion H1 ; auto.
+  * split ; intros ; assumption.
+  * destruct IHc_eq. split; intros ; auto. 
+  * destruct IHc_eq1. destruct IHc_eq2. split ; intros ; auto.
 Qed.
 
-Lemma plus_assoc : forall (c1 c2 c3 : Contract), ((c1 _+_ c2) _+_ c3) =R= (c1 _+_ (c2 _+_ c3)).
+
+Fixpoint monoms (c : Contract) : list Trace :=
+match c with
+| Success => [[]]
+| Failure => []
+| Event e => [[e]]
+| c0 _+_ c1 => (monoms c0) ++ (monoms c1)
+| c0 _;_ c1 => flat_map (fun m0 => map (fun m1 => m0 ++ m1) (monoms c1)) (monoms c0)
+end.
+
+Lemma monoms_seq : forall (s0 s1 s : Trace)(c0 c1 : Contract), In s0 (monoms c0) -> In s1 (monoms c1) -> In (s0++s1) (monoms (c0 _;_ c1)).
+Proof.
+intros. simpl. apply in_flat_map. exists s0. split. { assumption. }
+apply in_map. assumption.
+Qed. 
+
+
+
+Definition sorted_nodup_monoms_of_contract (c : Contract) : list Trace := sort ((nodup (list_eq_dec eq_event_dec)) (monoms c)).
+
+Definition contract_of_monom (s : Trace) := fold_left (fun acc e => acc _;_ (Event e)) s Success.
+
+
+Definition contract_of_monoms (l : list Trace) := fold_left (fun acc s => acc _+_ (contract_of_monom s)) l Failure.
+Compute (contract_of_monoms (monoms (Transfer _._  Notify _._ Success _+_ Notify _._ Success))).
+
+Definition norm_contract (c : Contract) : Contract := contract_of_monoms (sorted_nodup_monoms_of_contract c).
+
+(*Ltac unfold_norm_contract := unfold norm_contract, contract_of_monoms, sorted_nodup_monoms_of_contract.*)
+
+
+(*  Lemma incl_Forall_in_iff l l' :*)
+
+Lemma comp_equiv_destruct : forall (c0 c1: Contract),(forall s : Trace, s ==~ c0 <-> s ==~ c1) ->
+(forall s : Trace, s ==~ c0 -> s ==~ c1) /\ (forall s : Trace, s ==~ c1 -> s ==~ c0).
+Proof.
+intros. split ; intros; specialize H with s; destruct H; auto.
+Qed.
+
+Lemma norm_eq : forall (c: Contract), norm_contract c =R= c.
+Proof. Admitted.
+
+Lemma norm_match : forall (c: Contract), (forall s : Trace, s ==~ (norm_contract c) <-> s ==~ c).
+Proof.
+intro. apply c_eq_soundness. apply norm_eq.
+Qed.
+Check nodup.
+Lemma in_sorted_no_dump_monoms : forall (s : Trace)(c : Contract), In s (monoms c) -> 
+In s (sorted_nodup_monoms_of_contract c).
+Proof.
+intros. unfold sorted_nodup_monoms_of_contract. apply <- (nodup_In ((list_eq_dec eq_event_dec))) in H.
+remember (nodup (list_eq_dec eq_event_dec) (monoms c)) as l.
+apply Permutation_in with (l:=l). { apply Permuted_sort. } { assumption. }
+Qed.  
+
+
+Lemma match_member : forall (s : Trace)(c : Contract), s ==~ c <-> In s (monoms c). 
 Proof.
 split.
-- intro H. inversion H.
-  * inversion H2 ; auto. 
-  * auto.
-- intro H. inversion H.
-  * inversion H2 ; auto.
-  * inversion H1 ; auto.
-Qed.
+- intros. induction H ; try (simpl ; now left).
+  * apply monoms_seq; auto.
+  * simpl. apply in_or_app. now left.
+  * simpl. apply in_or_app. now right.
+- intros. apply (norm_match c s). unfold norm_contract. 
+  apply in_sorted_no_dump_monoms in H. unfold contract_of_monoms.
+  rewrite <- fold_left_rev_right.
+  
+    Admitted.
 
 
-Lemma seq_assoc : forall (c1 c2 c3 : Contract), ((c1 _;_ c2) _;_ c3) =R= (c1 _;_ (c2 _;_ c3)).
+Lemma comp_incl : forall (c0 c1 : Contract), (forall (s : Trace), s ==~ c0 -> s ==~ c1) -> 
+incl (monoms c0) (monoms c1).
 Proof.
-split.
-- intros. inversion H. inversion H3. rewrite <- app_assoc. all : auto.
-- intro H. inversion H. inversion H4. rewrite -> app_assoc. all : auto. 
-Qed.
-
-Lemma plus_or : forall (s : Trace)(c1 c2 : Contract), s ==~ (c1 _+_ c2) <-> s ==~ c1 \/ s ==~c2.
-Proof. 
-split.
-- intros. repeat rewrite comp_iff_oper in *. 
-apply plus_or_oper in H. assumption.
-- intros. destruct H; auto.
+intros. unfold incl. intros. apply match_member. apply H. apply match_member. assumption.
 Qed.
 
 
-Lemma plus_distr : forall (c1 c2 c3 : Contract), (c1 _;_ (c2 _+_ c3)) =R= (c1 _;_ c2) _+_ (c1 _;_ c3).
-Proof. split.
-- intros. inversion H ; inversion H4 ; auto.
-- intros. apply plus_or in H as [H | H] ; inversion H ; auto.
+Lemma sorted_permutation : forall (l1 l2 : list Trace), StronglySorted TraceOrder.leb_prop l1 -> StronglySorted TraceOrder.leb_prop l2 -> 
+Permutation l1 l2 -> l1 = l2.
+Proof.
+induction l1.
+- intros. apply Permutation_nil in H1. now rewrite H1.
+- intros. destruct l2.
+  * apply Permutation_sym in H1. apply Permutation_nil in H1. discriminate.
+  * inversion H. inversion H0. subst.
+    apply Permutation_in with (x:=a) in H1 as H10. 2: { now constructor. }
+    inversion H10.  { rewrite <- H2 in *. apply Permutation_cons_inv in H1. f_equal. auto. }
+    pose proof Permutation_sym H1 as H1_sym.
+    apply Permutation_in with (x:=t) in H1_sym as H11. 2: {  now constructor. }
+    inversion H11.  { rewrite <- H3 in *. apply Permutation_cons_inv in H1_sym. f_equal. apply Permutation_sym in H1_sym. auto. }
+    destruct (TraceOrder.leb_total a t). 
+    ** rewrite Forall_forall in H9. specialize H9 with a.
+       apply H9 in H2. unfold TraceOrder.leb_prop in H2.
+       destruct (TraceOrder.leb t a) eqn:Heqn. 2: { discriminate. }
+       pose proof TraceOrder.leb_anti_sym a t. unfold TraceOrder.leb_prop in H7.
+       rewrite Heqn in H7. rewrite H6 in H7. rewrite H7 in * ; auto. f_equal.
+       apply Permutation_cons_inv in H1. auto.
+    ** rewrite Forall_forall in H5. specialize H5 with t.
+       apply H5 in H3. unfold TraceOrder.leb_prop in H3.
+       destruct (TraceOrder.leb a t) eqn:Heqn.  2:{ discriminate. }
+       pose proof TraceOrder.leb_anti_sym t a. unfold TraceOrder.leb_prop in H7.
+       rewrite Heqn in H7. rewrite H6 in H7. rewrite H7 in * ; auto. f_equal.
+       apply Permutation_cons_inv in H1. auto.
 Qed.
 
-Lemma plus_distr2 : forall (c1 c2 c3 : Contract), ((c1 _+_ c2) _;_ c3) =R= (c1 _;_ c3) _+_ (c2 _;_ c3).
-Proof. split.
-- intros ; inversion H ; inversion H3 ; auto.
-- intros ; inversion H ; try inversion H2 ; try inversion H1 ; auto.
+
+Lemma comp_equiv_i_norm_eq : forall (c0 c1 : Contract), (forall s : Trace, s ==~ c0 <-> s ==~ c1) -> 
+forall (s' : Trace), In s' (monoms c0) <-> In s' (monoms c1).
+Proof.
+intros. apply comp_equiv_destruct with (c0:=c0)(c1:=c1) in H as [H1 H2].
+apply comp_incl in H1. apply comp_incl in H2. split ; auto.
+Qed.
+
+
+
+
+Search (Permutation _ _ -> _ ).
+Lemma comp_equiv_i_perm_monoms : forall (c0 c1 : Contract), (forall s : Trace, s ==~ c0 <-> s ==~ c1) -> 
+ Permutation (nodup (list_eq_dec eq_event_dec) (monoms c0)) 
+             (nodup (list_eq_dec eq_event_dec) (monoms c1)).
+Proof.
+intros. apply NoDup_Permutation ; try apply NoDup_nodup.
+intros. rewrite nodup_In. rewrite nodup_In. apply comp_equiv_i_norm_eq. assumption. 
+Qed.
+
+
+Lemma comp_equiv_i_eq_sorted_monoms : forall (c0 c1 : Contract), (forall s : Trace, s ==~ c0 <-> s ==~ c1) -> 
+ sorted_nodup_monoms_of_contract c0 = sorted_nodup_monoms_of_contract c1.
+Proof.
+intros. unfold sorted_nodup_monoms_of_contract. apply sorted_permutation.
+- apply (StronglySorted_sort ((nodup (list_eq_dec eq_event_dec) (monoms c0)) )TraceOrder.leb_trans).
+- apply (StronglySorted_sort ((nodup (list_eq_dec eq_event_dec) (monoms c1)) )TraceOrder.leb_trans).
+- repeat rewrite <- Permuted_sort. apply comp_equiv_i_perm_monoms. assumption.
+Qed.
+
+
+
+
+
+
+
+Lemma c_eq_completeness : forall (c0 c1 : Contract), (forall s : Trace, s ==~ c0 <-> s ==~ c1) -> c0 =R= c1.
+Proof.
+intros. rewrite <- norm_eq. rewrite <- (norm_eq c1). unfold norm_contract. f_equal. 
+apply comp_equiv_i_eq_sorted_monoms in H. rewrite H. apply c_refl.
 Qed.
